<?xml version="1.0"?>
<rdf:RDF xmlns="https://w3id.org/isoiec5087-2/v1/"
     xml:base="https://w3id.org/isoiec5087-2/v1/"
     xmlns:cc="http://creativecommons.org/ns#"
     xmlns:dcterms="http://purl.org/dc/terms/"
     xmlns:owl="http://www.w3.org/2002/07/owl#"
     xmlns:rdf="http://www.w3.org/1999/02/22-rdf-syntax-ns#"
     xmlns:rdfs="http://www.w3.org/2000/01/rdf-schema#"
     xmlns:skos="http://www.w3.org/2004/02/skos/core#"
     xmlns:vann="http://purl.org/vocab/vann/"
     xmlns:xml="http://www.w3.org/XML/1998/namespace"
     xmlns:xsd="http://www.w3.org/2001/XMLSchema#"
     xmlns:i72="https://w3id.org/isoiec21972/v1/"
     xmlns:cdm1="https://w3id.org/isoiec5087-1/v1/">
    <owl:Ontology rdf:about="https://w3id.org/isoiec5087-2/v1/CityResidentPattern">
        <!-- Identity -->
        <dcterms:title>Information technology - City data model - Part 2: City level concepts - City resident pattern</dcterms:title>
        <rdfs:seeAlso rdf:resource="https://www.iso.org/standard/80742.html"/>
        <dcterms:bibliographicCitation>ISO/IEC 5087-2:2024</dcterms:bibliographicCitation>
    	<skos:definition>This ontology specifies the city-level concepts for the city resident pattern of the city data model. As different cities have different definitions of who is that city's Resident, the City Resident Pattern must contain the properties required by each.  Central to all of the definitions is the concept of residing. Variously referred to as a home or domicile in which the resident spends significant amounts of time.  They may own it, rent it or just stay in it.  Legally, “reside means to dwell permanently or continuously. It expresses an idea that a person keeps or returns to a particular dwelling place as his fixed, settled, or legal abode. The meaning of reside implies a continuous arrangement” ; reside has both a temporal and spatial dimension. The city of Toronto's definition of a city resident includes the concept of owning property or owning or operating a business in the city. For Beijing, nationality is a unique aspect.</skos:definition>
    	<vann:preferredNamespaceUri>https://w3id.org/isoiec5087-2/v1/</vann:preferredNamespaceUri>
    	<vann:preferredNamespacePrefix>cdm2</vann:preferredNamespacePrefix>

    	<!-- Provenance -->
        <dcterms:creator>Megan Katsumi</dcterms:creator>
        <dcterms:creator>Mark Fox</dcterms:creator>
    	<dcterms:creator>Kenneth Vaughn</dcterms:creator>
        <dcterms:issued rdf:datatype="http://www.w3.org/2001/XMLSchema#date">2024</dcterms:issued> <!-- Date of the source document, comment out if draft -->
        <owl:priorVersion rdf:resource="https://standards.iso.org/iso-iec/5087/-2/ed-1/en/ontology/Building/"/>
        <owl:priorVersion rdf:datatype="http://www.w3.org/2001/XMLSchema#date">2021-01-11</owl:priorVersion> <!-- Date of prior ontology file, if any -->
		<dcterms:modified rdf:datatype="http://www.w3.org/2001/XMLSchema#date">2026-02-08</dcterms:modified> <!-- Date of this ontology file -->
        <owl:versionInfo>1.3.0</owl:versionInfo>
        <owl:versionIRI rdf:resource="https://w3id.org/isoiec5087-2/v1/r3.0"/>
        <rdfs:comment>The prior version of this ontology used a different ontology IRI. This update remains semantically consistent with the version adopted as ISO 5087-2:2024.</rdfs:comment>
        
        <!-- License -->
        <cc:license>http://creativecommons.org/licenses/by/4.0/</cc:license>
        
        <!-- Imports -->
        <owl:imports rdf:resource="https://w3id.org/isoiec5087-2/v1/BuildingPattern"/>
        <owl:imports rdf:resource="https://w3id.org/isoiec5087-2/v1/OrganizationPattern"/>
        <owl:imports rdf:resource="https://w3id.org/isoiec5087-2/v1/PersonPattern"/>
    </owl:Ontology>
    

    <!-- 
    ///////////////////////////////////////////////////////////////////////////////////////
    //
    // Object Properties
    //
    ///////////////////////////////////////////////////////////////////////////////////////
     -->

    
    <!-- https://w3id.org/isoiec5087-2/v1/CityResidentObjectProperty -->

    <owl:ObjectProperty rdf:about="https://w3id.org/isoiec5087-2/v1/CityResidentObjectProperty">
        <skos:definition>Added for organizational purposes, to identify object properties defined for the City Resident Pattern in the City-level CDM ontology.</skos:definition>
        <rdfs:subPropertyOf rdf:resource="https://w3id.org/isoiec5087-2/v1/CityObjectProperty"/>
    </owl:ObjectProperty>
    

    <!-- https://w3id.org/isoiec5087-2/v1/entity -->

    <owl:ObjectProperty rdf:about="https://w3id.org/isoiec5087-2/v1/entity">
        <skos:definition>Identifies an entity that is the subject domain object.</skos:definition>
        <skos:example>In the context of a ControlledEntity, the entity property would identify the entity being controlled.</skos:example>
        <rdfs:subPropertyOf rdf:resource="https://w3id.org/isoiec5087-2/v1/CityResidentObjectProperty"/>
    </owl:ObjectProperty>
    

    <!-- https://w3id.org/isoiec5087-2/v1/forCity -->

    <owl:ObjectProperty rdf:about="https://w3id.org/isoiec5087-2/v1/forCity">
        <skos:definition>Identifies the City of the residence.</skos:definition>
        <rdfs:subPropertyOf rdf:resource="https://w3id.org/isoiec5087-2/v1/CityResidentObjectProperty"/>
        <rdfs:domain rdf:resource="https://w3id.org/isoiec5087-2/v1/Residence"/>
        <rdfs:range rdf:resource="https://w3id.org/isoiec5087-2/v1/City"/>
    </owl:ObjectProperty>
    

    <!-- https://w3id.org/isoiec5087-2/v1/hasHomeType -->

    <owl:ObjectProperty rdf:about="https://w3id.org/isoiec5087-2/v1/hasHomeType">
        <skos:definition>Identifies the type of home.</skos:definition>
        <skos:example>house, apartment, or shelter</skos:example>
        <rdfs:subPropertyOf rdf:resource="https://w3id.org/isoiec5087-2/v1/CityResidentObjectProperty"/>
        <rdfs:domain rdf:resource="https://w3id.org/isoiec5087-2/v1/Residence"/>
        <rdfs:range rdf:resource="https://w3id.org/isoiec5087-2/v1/HomeType"/>
    </owl:ObjectProperty>
    

    <!-- https://w3id.org/isoiec5087-2/v1/hasResidence -->

    <owl:ObjectProperty rdf:about="https://w3id.org/isoiec5087-2/v1/hasResidence">
        <skos:definition>Specifies a Residence of a CityResident.</skos:definition>
        <rdfs:subPropertyOf rdf:resource="https://w3id.org/isoiec5087-2/v1/CityResidentObjectProperty"/>
        <rdfs:domain rdf:resource="https://w3id.org/isoiec5087-2/v1/CityResident"/>
        <rdfs:range rdf:resource="https://w3id.org/isoiec5087-2/v1/Residence"/>
    </owl:ObjectProperty>
    

    <!-- https://w3id.org/isoiec5087-2/v1/hasResidentialRelationship -->

    <owl:ObjectProperty rdf:about="https://w3id.org/isoiec5087-2/v1/hasResidentialRelationship">
        <skos:definition>Specifies the type of residential relationship that exists.</skos:definition>
        <skos:example>ownership, rental</skos:example>
        <rdfs:subPropertyOf rdf:resource="https://w3id.org/isoiec5087-2/v1/CityResidentObjectProperty"/>
        <rdfs:domain rdf:resource="https://w3id.org/isoiec5087-2/v1/Residence"/>
        <rdfs:range rdf:resource="https://w3id.org/isoiec5087-2/v1/ResidentialRelationship"/>
    </owl:ObjectProperty>
    

    <!-- https://w3id.org/isoiec5087-2/v1/operates -->

    <owl:ObjectProperty rdf:about="https://w3id.org/isoiec5087-2/v1/operates">
        <skos:definition>Specifies an EntityOperation where the entity is an Organization that the resident operates.</skos:definition>
        <rdfs:subPropertyOf rdf:resource="https://w3id.org/isoiec5087-2/v1/CityResidentObjectProperty"/>
        <rdfs:domain rdf:resource="https://w3id.org/isoiec5087-2/v1/CityResident"/>
        <rdfs:range rdf:resource="https://w3id.org/isoiec5087-2/v1/EntityOperation"/>
    </owl:ObjectProperty>
    

    <!-- https://w3id.org/isoiec5087-2/v1/owns -->

    <owl:ObjectProperty rdf:about="https://w3id.org/isoiec5087-2/v1/owns">
        <skos:definition>Identifies an entity that is owned by another entity.</skos:definition>
        <rdfs:subPropertyOf rdf:resource="https://w3id.org/isoiec5087-2/v1/CityResidentObjectProperty"/>
        <rdfs:range rdf:resource="https://w3id.org/isoiec5087-2/v1/EntityOwnership"/>
    </owl:ObjectProperty>
    

    <!-- https://w3id.org/isoiec5087-2/v1/residentOf -->

    <owl:ObjectProperty rdf:about="https://w3id.org/isoiec5087-2/v1/residentOf">
        <skos:definition>Identifies the JurisdictionalArea that a CityResident is a resident.</skos:definition>
        <rdfs:subPropertyOf rdf:resource="https://w3id.org/isoiec5087-2/v1/CityResidentObjectProperty"/>
        <rdfs:domain rdf:resource="https://w3id.org/isoiec5087-2/v1/CityResident"/>
        <rdfs:range rdf:resource="https://w3id.org/isoiec5087-2/v1/JurisdictionalArea"/>
    </owl:ObjectProperty>
    

    <!-- 
    ///////////////////////////////////////////////////////////////////////////////////////
    //
    // Data properties
    //
    ///////////////////////////////////////////////////////////////////////////////////////
     -->

    
    <!-- https://w3id.org/isoiec5087-2/v1/CityResidentDataProperty -->

    <owl:DatatypeProperty rdf:about="https://w3id.org/isoiec5087-2/v1/CityResidentDataProperty">
        <skos:definition>Added for organizational purposes, to identify data properties defined in the City Resident Pattern.</skos:definition>
        <rdfs:subPropertyOf rdf:resource="https://w3id.org/isoiec5087-2/v1/CityDataProperty"/>
    </owl:DatatypeProperty>
    

    <!-- https://w3id.org/isoiec5087-2/v1/percentOwnership -->

    <owl:DatatypeProperty rdf:about="https://w3id.org/isoiec5087-2/v1/percentOwnership">
        <skos:definition>Specifies the percentage of ownership that an entity has in another entity.</skos:definition>
        <rdfs:subPropertyOf rdf:resource="https://w3id.org/isoiec5087-2/v1/CityResidentDataProperty"/>
        <rdfs:domain rdf:resource="https://w3id.org/isoiec5087-2/v1/EntityOwnership"/>
        <rdfs:range rdf:resource="http://www.w3.org/2001/XMLSchema#decimal"/>
    </owl:DatatypeProperty>
    

    <!-- 
    ///////////////////////////////////////////////////////////////////////////////////////
    //
    // Classes
    //
    ///////////////////////////////////////////////////////////////////////////////////////
     -->

    
    <!-- https://w3id.org/isoiec5087-2/v1/CityResidentThing -->

    <owl:Class rdf:about="https://w3id.org/isoiec5087-2/v1/CityResidentThing">
        <rdfs:subClassOf rdf:resource="https://w3id.org/isoiec5087-2/v1/CityThing"/>
        <skos:definition>Added for organizational purposes, to identify classes defined in the City Resident ontology.</skos:definition>
    </owl:Class>
    

    <!-- https://w3id.org/isoiec5087-2/v1/CityResident -->

    <owl:Class rdf:about="https://w3id.org/isoiec5087-2/v1/CityResident">
        <skos:definition>A City Resident is a Person who satisfies the requirements of being a city resident for the particular City.</skos:definition>
        <skos:note>Different cities have different definitions of who is that city's Resident, the City Resident Pattern contains the core properties required by each. For example, the city of Toronto's definition of a city resident includes the concept of owning property or owning or operating a business in the city. For Beijing, nationality is a unique aspect. Central to all the definitions is the concept of residing. </skos:note>
        <rdfs:subClassOf rdf:resource="https://w3id.org/isoiec5087-2/v1/CityResidentThing"/>
        <rdfs:subClassOf rdf:resource="https://w3id.org/isoiec5087-2/v1/Person"/>
        <rdfs:subClassOf>
            <owl:Restriction>
                <owl:onProperty rdf:resource="https://w3id.org/isoiec5087-2/v1/hasResidence"/>
                <owl:allValuesFrom rdf:resource="https://w3id.org/isoiec5087-2/v1/Residence"/>
            </owl:Restriction>
        </rdfs:subClassOf>
        <rdfs:subClassOf>
            <owl:Restriction>
                <owl:onProperty rdf:resource="https://w3id.org/isoiec5087-2/v1/operates"/>
                <owl:allValuesFrom rdf:resource="https://w3id.org/isoiec5087-2/v1/EntityOperation"/>
            </owl:Restriction>
        </rdfs:subClassOf>
        <rdfs:subClassOf>
            <owl:Restriction>
                <owl:onProperty rdf:resource="https://w3id.org/isoiec5087-2/v1/owns"/>
                <owl:allValuesFrom rdf:resource="https://w3id.org/isoiec5087-2/v1/EntityOwnership"/>
            </owl:Restriction>
        </rdfs:subClassOf>
        <rdfs:subClassOf>
            <owl:Restriction>
                <owl:onProperty rdf:resource="https://w3id.org/isoiec5087-2/v1/residentOf"/>
                <owl:allValuesFrom rdf:resource="https://w3id.org/isoiec5087-2/v1/JurisdictionalArea"/>
            </owl:Restriction>
        </rdfs:subClassOf>
    </owl:Class>
    

    <!-- https://w3id.org/isoiec5087-2/v1/ControlledEntity -->

    <owl:Class rdf:about="https://w3id.org/isoiec5087-2/v1/ControlledEntity">
        <skos:definition>A controlled entity is an entity that is subject to control by another entity.</skos:definition>
        <rdfs:subClassOf rdf:resource="https://w3id.org/isoiec5087-2/v1/CityResidentThing"/>
        <rdfs:subClassOf>
            <owl:Restriction>
                <owl:onProperty rdf:resource="https://w3id.org/isoiec5087-2/v1/entity"/>
                <owl:someValuesFrom rdf:resource="http://www.w3.org/2002/07/owl#Thing"/>
            </owl:Restriction>
        </rdfs:subClassOf>
        <rdfs:subClassOf>
            <owl:Restriction>
                <owl:onProperty rdf:resource="http://www.w3.org/2006/time#hasTime"/>
                <owl:maxQualifiedCardinality rdf:datatype="http://www.w3.org/2001/XMLSchema#nonNegativeInteger">1</owl:maxQualifiedCardinality>
                <owl:onClass rdf:resource="http://www.w3.org/2006/time#ProperInterval"/>
            </owl:Restriction>
        </rdfs:subClassOf>
    </owl:Class>
    

    <!-- https://w3id.org/isoiec5087-2/v1/EntityOperation -->

    <owl:Class rdf:about="https://w3id.org/isoiec5087-2/v1/EntityOperation">
        <skos:definition>Activity of operating an Organization by City Resident.</skos:definition>
        <rdfs:subClassOf rdf:resource="https://w3id.org/isoiec5087-2/v1/ControlledEntity"/>
        <rdfs:subClassOf>
            <owl:Restriction>
                <owl:onProperty rdf:resource="https://w3id.org/isoiec5087-2/v1/entity"/>
                <owl:maxQualifiedCardinality rdf:datatype="http://www.w3.org/2001/XMLSchema#nonNegativeInteger">1</owl:maxQualifiedCardinality>
                <owl:onClass rdf:resource="https://w3id.org/isoiec5087-2/v1/Organization"/>
            </owl:Restriction>
        </rdfs:subClassOf>
    </owl:Class>
    

    <!-- https://w3id.org/isoiec5087-2/v1/EntityOwnership -->

    <owl:Class rdf:about="https://w3id.org/isoiec5087-2/v1/EntityOwnership">
        <skos:definition>Activity of owning a Building, Land Area, or Organization by City Resident.</skos:definition>
        <rdfs:subClassOf rdf:resource="https://w3id.org/isoiec5087-2/v1/ControlledEntity"/>
        <rdfs:subClassOf>
            <owl:Restriction>
                <owl:onProperty rdf:resource="https://w3id.org/isoiec5087-2/v1/entity"/>
                <owl:maxQualifiedCardinality rdf:datatype="http://www.w3.org/2001/XMLSchema#nonNegativeInteger">1</owl:maxQualifiedCardinality>
                <owl:onClass>
                    <owl:Class>
                        <owl:unionOf rdf:parseType="Collection">
                            <rdf:Description rdf:about="https://w3id.org/isoiec5087-2/v1/Building"/>
                            <rdf:Description rdf:about="https://w3id.org/isoiec5087-2/v1/LandArea"/>
                            <rdf:Description rdf:about="https://w3id.org/isoiec5087-2/v1/Organization"/>
                        </owl:unionOf>
                    </owl:Class>
                </owl:onClass>
            </owl:Restriction>
        </rdfs:subClassOf>
        <rdfs:subClassOf>
            <owl:Restriction>
                <owl:onProperty rdf:resource="https://w3id.org/isoiec5087-2/v1/percentOwnership"/>
                <owl:maxQualifiedCardinality rdf:datatype="http://www.w3.org/2001/XMLSchema#nonNegativeInteger">1</owl:maxQualifiedCardinality>
                <owl:onDataRange rdf:resource="http://www.w3.org/2001/XMLSchema#decimal"/>
            </owl:Restriction>
        </rdfs:subClassOf>
    </owl:Class>
    

    <!-- https://w3id.org/isoiec5087-2/v1/HomeType -->

    <owl:Class rdf:about="https://w3id.org/isoiec5087-2/v1/HomeType">
        <skos:definition>Home Type is a type of Code that describes the type of a Residence.</skos:definition>
        <rdfs:subClassOf rdf:resource="https://w3id.org/isoiec5087-2/v1/CityResidentThing"/>
        <rdfs:subClassOf>
            <owl:Restriction>
                <owl:onProperty rdf:resource="https://w3id.org/isoiec5087-2/v1/hasCode"/>
                <owl:allValuesFrom rdf:resource="https://w3id.org/isoiec5087-2/v1/Code"/>
            </owl:Restriction>
        </rdfs:subClassOf>
    </owl:Class>
    

    <!-- https://w3id.org/isoiec5087-2/v1/Residence -->

    <owl:Class rdf:about="https://w3id.org/isoiec5087-2/v1/Residence">
        <rdfs:subClassOf rdf:resource="https://w3id.org/isoiec5087-2/v1/CityResidentThing"/>
        <!-- Issue: ISO/IEC 5087-2 defines hasResidentialRelationship as max 1 rather exactly 1; keep for max 1 for now as it can be broadened to only if needed. -->
        <rdfs:subClassOf>
            <owl:Restriction>
                <owl:onProperty rdf:resource="https://w3id.org/isoiec5087-2/v1/hasResidentialRelationship"/>
                <owl:qualifiedCardinality rdf:datatype="http://www.w3.org/2001/XMLSchema#nonNegativeInteger">1</owl:qualifiedCardinality>
                <owl:onClass rdf:resource="https://w3id.org/isoiec5087-2/v1/ResidentialRelationship"/>
            </owl:Restriction>
        </rdfs:subClassOf>
        <rdfs:subClassOf>
            <owl:Restriction>
                <owl:onProperty rdf:resource="https://w3id.org/isoiec5087-2/v1/forCity"/>
                <owl:maxQualifiedCardinality rdf:datatype="http://www.w3.org/2001/XMLSchema#nonNegativeInteger">1</owl:maxQualifiedCardinality>
                <owl:onClass rdf:resource="https://w3id.org/isoiec5087-2/v1/City"/>
            </owl:Restriction>
        </rdfs:subClassOf>
        <rdfs:subClassOf>
            <owl:Restriction>
                <owl:onProperty rdf:resource="https://w3id.org/isoiec5087-2/v1/hasHomeType"/>
                <owl:maxQualifiedCardinality rdf:datatype="http://www.w3.org/2001/XMLSchema#nonNegativeInteger">1</owl:maxQualifiedCardinality>
                <owl:onClass rdf:resource="https://w3id.org/isoiec5087-2/v1/HomeType"/>
            </owl:Restriction>
        </rdfs:subClassOf>
        <rdfs:subClassOf>
            <owl:Restriction>
                <owl:onProperty rdf:resource="https://w3id.org/isoiec5087-2/v1/hasAddress"/>
                <owl:maxQualifiedCardinality rdf:datatype="http://www.w3.org/2001/XMLSchema#nonNegativeInteger">1</owl:maxQualifiedCardinality>
                <owl:onClass rdf:resource="https://w3id.org/isoiec5087-2/v1/Address"/>
            </owl:Restriction>
        </rdfs:subClassOf>
        <rdfs:subClassOf>
            <owl:Restriction>
                <owl:onProperty rdf:resource="http://www.w3.org/2006/time#hasTime"/>
                <owl:maxQualifiedCardinality rdf:datatype="http://www.w3.org/2001/XMLSchema#nonNegativeInteger">1</owl:maxQualifiedCardinality>
                <owl:onClass rdf:resource="http://www.w3.org/2006/time#ProperInterval"/>
            </owl:Restriction>
        </rdfs:subClassOf>
    </owl:Class>
    

<!-- Issue: ISO/IEC 5087-2 does not define hasResidentialRelationship but references it. Keep. -->
    <!-- https://w3id.org/isoiec5087-2/v1/ResidentialRelationship -->

    <owl:Class rdf:about="https://w3id.org/isoiec5087-2/v1/ResidentialRelationship">
        <skos:definition>A ResidentialRelationship defines the relationship of a Resident to a Residence.</skos:definition>
        <rdfs:subClassOf rdf:resource="https://w3id.org/isoiec5087-2/v1/CityResidentThing"/>
        <rdfs:subClassOf>
            <owl:Restriction>
                <owl:onProperty rdf:resource="https://w3id.org/isoiec5087-2/v1/hasCode"/>
                <owl:allValuesFrom rdf:resource="https://w3id.org/isoiec5087-2/v1/Code"/>
            </owl:Restriction>
        </rdfs:subClassOf>
    </owl:Class>
    

    <!-- 
    ///////////////////////////////////////////////////////////////////////////////////////
    //
    // Individuals
    //
    ///////////////////////////////////////////////////////////////////////////////////////
     -->

    


    <!-- https://w3id.org/isoiec5087-2/v1/apartment -->

    <owl:NamedIndividual rdf:about="https://w3id.org/isoiec5087-2/v1/apartment"/>
    


    <!-- https://w3id.org/isoiec5087-2/v1/condominium -->

    <owl:NamedIndividual rdf:about="https://w3id.org/isoiec5087-2/v1/condominium"/>
    


    <!-- https://w3id.org/isoiec5087-2/v1/freeload -->

    <owl:NamedIndividual rdf:about="https://w3id.org/isoiec5087-2/v1/freeload"/>
    


    <!-- https://w3id.org/isoiec5087-2/v1/hotel -->

    <owl:NamedIndividual rdf:about="https://w3id.org/isoiec5087-2/v1/hotel"/>
    


    <!-- https://w3id.org/isoiec5087-2/v1/house -->

    <owl:NamedIndividual rdf:about="https://w3id.org/isoiec5087-2/v1/house"/>
    


    <!-- https://w3id.org/isoiec5087-2/v1/lease -->

    <owl:NamedIndividual rdf:about="https://w3id.org/isoiec5087-2/v1/lease"/>
    


    <!-- https://w3id.org/isoiec5087-2/v1/openLand -->

    <owl:NamedIndividual rdf:about="https://w3id.org/isoiec5087-2/v1/openLand"/>
    


    <!-- https://w3id.org/isoiec5087-2/v1/own -->

    <owl:NamedIndividual rdf:about="https://w3id.org/isoiec5087-2/v1/own"/>
    


    <!-- https://w3id.org/isoiec5087-2/v1/rent -->

    <owl:NamedIndividual rdf:about="https://w3id.org/isoiec5087-2/v1/rent"/>
    


    <!-- https://w3id.org/isoiec5087-2/v1/rent-to-own -->

    <owl:NamedIndividual rdf:about="https://w3id.org/isoiec5087-2/v1/rent-to-own"/>
    


    <!-- https://w3id.org/isoiec5087-2/v1/shelter -->

    <owl:NamedIndividual rdf:about="https://w3id.org/isoiec5087-2/v1/shelter"/>
</rdf:RDF>
