<?xml version="1.0"?>
<rdf:RDF xmlns="https://w3id.org/citydata/part2/v1/"
     xml:base="https://w3id.org/citydata/part2/v1/"
     xmlns:cc="http://creativecommons.org/ns#"
     xmlns:dcterms="http://purl.org/dc/terms/"
     xmlns:owl="http://www.w3.org/2002/07/owl#"
     xmlns:rdf="http://www.w3.org/1999/02/22-rdf-syntax-ns#"
     xmlns:rdfs="http://www.w3.org/2000/01/rdf-schema#"
     xmlns:skos="http://www.w3.org/2004/02/skos/core#"
     xmlns:vann="http://purl.org/vocab/vann/"
     xmlns:xml="http://www.w3.org/XML/1998/namespace"
     xmlns:xsd="http://www.w3.org/2001/XMLSchema#"
     xmlns:cdm1="https://w3id.org/citydata/part1/v1/">
    <owl:Ontology rdf:about="https://w3id.org/citydata/part2/v1/ContractPattern/">
        <!-- Identity -->
        <dcterms:title>Information technology - City data model - Part 2: City level concepts - Contract pattern</dcterms:title>
        <rdfs:seeAlso rdf:resource="https://www.iso.org/standard/80742.html"/>
        <dcterms:bibliographicCitation>ISO/IEC 5087-2:2024</dcterms:bibliographicCitation>
    	<skos:definition>This ontology specifies the city-level concepts for the contract pattern of the city data model. A contract is a legal document that specifies some agreement(s) between two or more parties. The aim of the contract pattern is not to formalize the semantics of all possible involved legal concepts, but rather to enable to representation of the general structure and contents of a particular contract. The Contract Ontology adopts the definition of Contract specified in the Financial Business Ontology (FIBO) [8] specified at: https://spec.edmcouncil.org/fibo/ontology/FND/Agreements/Contracts/ with a key modification that a Contract is defined as a type of Document and is distinct from an Agreement (not a subclass, as specified in FIBO).</skos:definition>
    	<vann:preferredNamespaceUri>https://w3id.org/citydata/part2/v1/</vann:preferredNamespaceUri>
    	<vann:preferredNamespacePrefix>cdm2</vann:preferredNamespacePrefix>

    	<!-- Provenance -->
        <dcterms:creator>Megan Katsumi</dcterms:creator>
        <dcterms:creator>Mark Fox</dcterms:creator>
    	<dcterms:creator>Kenneth Vaughn</dcterms:creator>
        <!-- Prior release -->
        <rdfs:comment>The prior version of this ontology used a different ontology IRI. This update remains semantically consistent with the version adopted as ISO 5087-2:2024.</rdfs:comment>
        <owl:priorVersion rdf:resource="https://standards.iso.org/iso-iec/5087/-2/ed-1/en/ontology/Contract/"/>
        <!-- This release -->
		<dcterms:modified rdf:datatype="http://www.w3.org/2001/XMLSchema#date">2026-02-12</dcterms:modified> 
        <owl:versionInfo>1.3.0</owl:versionInfo>
        <owl:versionIRI rdf:resource="https://w3id.org/citydata/part2/v1/ContractPattern/r3.0/"/>
        
        <!-- License -->
        <cc:license>http://creativecommons.org/licenses/by/4.0/</cc:license>
        
        <!-- Imports -->
        <owl:imports rdf:resource="https://w3id.org/citydata/part1/v1/AgreementPattern/"/>
        <owl:imports rdf:resource="https://w3id.org/citydata/part2/v1/OrganizationPattern/"/>
    </owl:Ontology>
    

   <!-- 
    ///////////////////////////////////////////////////////////////////////////////////////
    //
    // Object Properties
    //
    ///////////////////////////////////////////////////////////////////////////////////////
     -->

    
    <!-- https://w3id.org/citydata/part2/v1/ContractObjectProperty -->

    <owl:ObjectProperty rdf:about="https://w3id.org/citydata/part2/v1/ContractObjectProperty">
        <skos:definition>Added for organizational purposes, to identify object properties defined for the Contract Pattern in the City-level CDM ontology.</skos:definition>
        <rdfs:subPropertyOf rdf:resource="https://w3id.org/citydata/part2/v1/CityObjectProperty"/>
    </owl:ObjectProperty>
    

    <!-- https://w3id.org/citydata/part2/v1/hasContract -->

    <owl:ObjectProperty rdf:about="https://w3id.org/citydata/part2/v1/hasContract">
        <skos:definition>Identifies the Contract associated with the domain object.</skos:definition>
        <rdfs:subPropertyOf rdf:resource="https://w3id.org/citydata/part2/v1/ContractObjectProperty"/>
        <rdfs:range rdf:resource="https://w3id.org/citydata/part2/v1/Contract"/>
    </owl:ObjectProperty>
    

    <!-- https://w3id.org/citydata/part2/v1/hasContractualElement -->

    <owl:ObjectProperty rdf:about="https://w3id.org/citydata/part2/v1/hasContractualElement">
        <skos:definition>Identifies the decomposition of a Contract into more precise parts.</skos:definition>
        <rdfs:subPropertyOf rdf:resource="https://w3id.org/citydata/part2/v1/ContractObjectProperty"/>
        <rdfs:subPropertyOf rdf:resource="https://w3id.org/citydata/part1/v1/hasComponent"/>
        <rdfs:domain rdf:resource="https://w3id.org/citydata/part2/v1/Contract"/>
        <rdfs:range rdf:resource="https://w3id.org/citydata/part2/v1/ContractualElement"/>
    </owl:ObjectProperty>
    

    <!-- https://w3id.org/citydata/part2/v1/hasParty -->

    <owl:ObjectProperty rdf:about="https://w3id.org/citydata/part2/v1/hasParty">
        <skos:definition>Identifies all Persons or Organizations involved in the Contract.</skos:definition>
        <rdfs:subPropertyOf rdf:resource="https://w3id.org/citydata/part2/v1/ContractObjectProperty"/>
        <rdfs:range rdf:resource="https://w3id.org/citydata/part1/v1/Agent"/>
    </owl:ObjectProperty>
    

    <!-- https://w3id.org/citydata/part2/v1/hasSignatory -->

    <owl:ObjectProperty rdf:about="https://w3id.org/citydata/part2/v1/hasSignatory">
        <skos:definition>identifies the Person(s) responsible for signing the Contract.</skos:definition>
        <rdfs:subPropertyOf rdf:resource="https://w3id.org/citydata/part2/v1/ContractObjectProperty"/>
        <rdfs:domain rdf:resource="https://w3id.org/citydata/part2/v1/Contract"/>
        <rdfs:range rdf:resource="https://w3id.org/citydata/part2/v1/Person"/>
    </owl:ObjectProperty>
    

    <!-- Issue: v1.2.0 defined executedOn; revised to isExecutedOn to align with ISO/IEC 5087-2 -->
    <!-- https://w3id.org/citydata/part2/v1/isExecutedOn -->

    <owl:ObjectProperty rdf:about="https://w3id.org/citydata/part2/v1/isExecutedOn">
        <skos:definition>identifies the Interval or Instant in time at which the terms in the Contract are executed, if applicable.</skos:definition>
        <rdfs:subPropertyOf rdf:resource="https://w3id.org/citydata/part2/v1/ContractObjectProperty"/>
        <rdfs:domain rdf:resource="https://w3id.org/citydata/part2/v1/Contract"/>
        <rdfs:range rdf:resource="http://www.w3.org/2006/time#TemporalEntity"/>
    </owl:ObjectProperty>
    

    <!-- https://w3id.org/citydata/part2/v1/isValidFor -->

    <owl:ObjectProperty rdf:about="https://w3id.org/citydata/part2/v1/isValidFor">
        <skos:definition>Identifies the Interval in time over which the domain object is valid.</skos:definition>
        <rdfs:subPropertyOf rdf:resource="https://w3id.org/citydata/part2/v1/ContractObjectProperty"/>
        <rdfs:range rdf:resource="http://www.w3.org/2006/time#TimeInterval"/>
    </owl:ObjectProperty>
    

    <!-- https://w3id.org/citydata/part2/v1/specifiesAgreement -->

    <owl:ObjectProperty rdf:about="https://w3id.org/citydata/part2/v1/specifiesAgreement">
        <skos:definition>Identifies an agreement that is specified by the domain object.</skos:definition>
        <rdfs:subPropertyOf rdf:resource="https://w3id.org/citydata/part2/v1/ContractObjectProperty"/>
        <rdfs:range rdf:resource="https://w3id.org/citydata/part1/v1/Agreement"/>
    </owl:ObjectProperty>
    

    <!-- 
    ///////////////////////////////////////////////////////////////////////////////////////
    //
    // Data properties
    //
    ///////////////////////////////////////////////////////////////////////////////////////
     -->

    
    <!-- https://w3id.org/citydata/part2/v1/ContractDataProperty -->

    <owl:DatatypeProperty rdf:about="https://w3id.org/citydata/part2/v1/ContractDataProperty">
        <skos:definition>Added for organizational purposes, to identify data properties defined in the Contract Pattern.</skos:definition>
        <rdfs:subPropertyOf rdf:resource="https://w3id.org/citydata/part2/v1/CityDataProperty"/>
    </owl:DatatypeProperty>
    

    <!-- https://w3id.org/citydata/part2/v1/hasContractText -->

    <owl:DatatypeProperty rdf:about="https://w3id.org/citydata/part2/v1/hasContractText">
        <skos:definition>Identifies the excerpt of text from the Contract that corresponds to the Contractual Element.</skos:definition>
        <rdfs:subPropertyOf rdf:resource="https://w3id.org/citydata/part2/v1/ContractDataProperty"/>
        <rdfs:domain rdf:resource="https://w3id.org/citydata/part2/v1/ContractualElement"/>
        <rdfs:range rdf:resource="http://www.w3.org/2001/XMLSchema#string"/>
    </owl:DatatypeProperty>
    

    <!-- 
    ///////////////////////////////////////////////////////////////////////////////////////
    //
    // Classes
    //
    ///////////////////////////////////////////////////////////////////////////////////////
     -->

    
    <!-- https://w3id.org/citydata/part2/v1/ContractThing -->

    <owl:Class rdf:about="https://w3id.org/citydata/part2/v1/ContractThing">
        <rdfs:subClassOf rdf:resource="https://w3id.org/citydata/part2/v1/CityThing"/>
        <skos:definition>Added for organizational purposes, to identify classes defined in the Contract ontology.</skos:definition>
    </owl:Class>
    

    <!-- https://w3id.org/citydata/part2/v1/ConditionPrecedent -->

    <owl:Class rdf:about="https://w3id.org/citydata/part2/v1/ConditionPrecedent">
        <skos:definition>A condition precedent is a condition that must be met before a contract becomes effective.</skos:definition>
        <rdfs:subClassOf rdf:resource="https://w3id.org/citydata/part2/v1/ContractualElement"/>
    </owl:Class>
    

    <!-- https://w3id.org/citydata/part2/v1/Contract -->

    <owl:Class rdf:about="https://w3id.org/citydata/part2/v1/Contract">
        <skos:definition>A contract is a legally binding agreement between two or more parties.</skos:definition>
        <rdfs:subClassOf rdf:resource="https://w3id.org/citydata/part2/v1/ContractThing"/>
        <rdfs:subClassOf>
            <owl:Restriction>
                <owl:onProperty rdf:resource="https://w3id.org/citydata/part2/v1/hasContractualElement"/>
                <owl:someValuesFrom rdf:resource="https://w3id.org/citydata/part2/v1/ContractualElement"/>
            </owl:Restriction>
        </rdfs:subClassOf>
        <rdfs:subClassOf>
            <owl:Restriction>
                <owl:onProperty rdf:resource="https://w3id.org/citydata/part2/v1/specifiesAgreement"/>
                <owl:someValuesFrom rdf:resource="https://w3id.org/citydata/part1/v1/Agreement"/>
            </owl:Restriction>
        </rdfs:subClassOf>
        <!-- Issue: ISO/IEC 5087-2 uses the term "isExecutedOn" for executedOn. Recommend isExecutedOn. -->
        <rdfs:subClassOf>
            <owl:Restriction>
                <owl:onProperty rdf:resource="https://w3id.org/citydata/part2/v1/isExecutedOn"/>
                <owl:allValuesFrom rdf:resource="http://www.w3.org/2006/time#TemporalEntity"/>
            </owl:Restriction>
        </rdfs:subClassOf>
        <rdfs:subClassOf>
            <owl:Restriction>
                <owl:onProperty rdf:resource="https://w3id.org/citydata/part2/v1/isValidFor"/>
                <owl:allValuesFrom rdf:resource="http://www.w3.org/2006/time#Interval"/>
            </owl:Restriction>
        </rdfs:subClassOf>
        <rdfs:subClassOf>
            <owl:Restriction>
                <owl:onProperty rdf:resource="https://w3id.org/citydata/part2/v1/hasParty"/>
                <owl:minQualifiedCardinality rdf:datatype="http://www.w3.org/2001/XMLSchema#nonNegativeInteger">2</owl:minQualifiedCardinality>
                <owl:onClass>
                    <owl:Class>
                        <owl:unionOf rdf:parseType="Collection">
                            <rdf:Description rdf:about="https://w3id.org/citydata/part2/v1/Organization"/>
                            <rdf:Description rdf:about="https://w3id.org/citydata/part2/v1/Person"/>
                        </owl:unionOf>
                    </owl:Class>
                </owl:onClass>
            </owl:Restriction>
        </rdfs:subClassOf>
        <rdfs:subClassOf>
            <owl:Restriction>
                <owl:onProperty rdf:resource="https://w3id.org/citydata/part2/v1/hasSignatory"/>
                <owl:minQualifiedCardinality rdf:datatype="http://www.w3.org/2001/XMLSchema#nonNegativeInteger">2</owl:minQualifiedCardinality>
                <owl:onClass rdf:resource="https://w3id.org/citydata/part2/v1/Person"/>
            </owl:Restriction>
        </rdfs:subClassOf>
    </owl:Class>
    

    <!-- https://w3id.org/citydata/part2/v1/ContractualCommitment -->

    <owl:Class rdf:about="https://w3id.org/citydata/part2/v1/ContractualCommitment">
        <skos:definition>A contractual commitment is a legally binding part of a contract that consists of a promise made by a party in relation to the contract.</skos:definition>
        <rdfs:subClassOf rdf:resource="https://w3id.org/citydata/part2/v1/ContractualElement"/>
        <!-- Issue: ISO/IEC 5087-2 defines specifiesAgreement some Agreement rather than only Agreement. Change to some. -->
        <rdfs:subClassOf>
            <owl:Restriction>
                <owl:onProperty rdf:resource="https://w3id.org/citydata/part2/v1/specifiesAgreement"/>
                <owl:allValuesFrom rdf:resource="https://w3id.org/citydata/part1/v1/Agreement"/>
            </owl:Restriction>
        </rdfs:subClassOf>
    </owl:Class>
    

    <!-- https://w3id.org/citydata/part2/v1/ContractualDefinition -->

    <owl:Class rdf:about="https://w3id.org/citydata/part2/v1/ContractualDefinition">
        <skos:definition>A contractual definition is a definition of a term used within a contract.</skos:definition>
        <rdfs:subClassOf rdf:resource="https://w3id.org/citydata/part2/v1/ContractualElement"/>
    </owl:Class>
    

    <!-- https://w3id.org/citydata/part2/v1/ContractualElement -->

    <owl:Class rdf:about="https://w3id.org/citydata/part2/v1/ContractualElement">
        <skos:definition>A contractual element is an element that forms part of a contract, such as a definition, condition, or commitment.</skos:definition>
        <rdfs:subClassOf rdf:resource="https://w3id.org/citydata/part2/v1/ContractThing"/>
        <rdfs:subClassOf>
            <owl:Restriction>
                <owl:onProperty>
                    <rdf:Description>
                        <owl:inverseOf rdf:resource="https://w3id.org/citydata/part2/v1/hasContractualElement"/>
                    </rdf:Description>
                </owl:onProperty>
                <owl:someValuesFrom rdf:resource="https://w3id.org/citydata/part2/v1/Contract"/>
            </owl:Restriction>
        </rdfs:subClassOf>
        <rdfs:subClassOf>
            <owl:Restriction>
                <owl:onProperty rdf:resource="https://w3id.org/citydata/part2/v1/hasContractText"/>
                <owl:someValuesFrom rdf:resource="http://www.w3.org/2001/XMLSchema#string"/>
            </owl:Restriction>
        </rdfs:subClassOf>
    </owl:Class>
    

    <!-- https://w3id.org/citydata/part2/v1/NonBindingTerm -->

    <owl:Class rdf:about="https://w3id.org/citydata/part2/v1/NonBindingTerm">
        <skos:definition>A NonBindingTerm is a term in a contract that does not have legal force.</skos:definition>
        <rdfs:subClassOf rdf:resource="https://w3id.org/citydata/part2/v1/ContractualElement"/>
    </owl:Class>
    

    <!-- https://w3id.org/citydata/part2/v1/Representation -->

    <owl:Class rdf:about="https://w3id.org/citydata/part2/v1/Representation">
        <skos:definition>Part of the Contract that specifies some assertions that are taken to be true at the time of the contract and serve to influence a party's decision to enter into the Contract.</skos:definition>
        <rdfs:subClassOf rdf:resource="https://w3id.org/citydata/part2/v1/ContractualElement"/>
    </owl:Class>
    

    <!-- https://w3id.org/citydata/part2/v1/Warranty -->

    <owl:Class rdf:about="https://w3id.org/citydata/part2/v1/Warranty">
        <skos:definition>A Warranty is a contractual promise of some indemnification if an assertion made in the Contract is false.</skos:definition>
        <rdfs:subClassOf rdf:resource="https://w3id.org/citydata/part2/v1/ContractualElement"/>
    </owl:Class>


</rdf:RDF>
