<?xml version="1.0"?>
<rdf:RDF xmlns="https://w3id.org/citydata/part2/v1/"
     xml:base="https://w3id.org/citydata/part2/v1/"
     xmlns:cc="http://creativecommons.org/ns#"
     xmlns:dcterms="http://purl.org/dc/terms/"
     xmlns:owl="http://www.w3.org/2002/07/owl#"
     xmlns:rdf="http://www.w3.org/1999/02/22-rdf-syntax-ns#"
     xmlns:rdfs="http://www.w3.org/2000/01/rdf-schema#"
     xmlns:skos="http://www.w3.org/2004/02/skos/core#"
     xmlns:vann="http://purl.org/vocab/vann/"
     xmlns:xml="http://www.w3.org/XML/1998/namespace"
     xmlns:xsd="http://www.w3.org/2001/XMLSchema#"
     xmlns:i72="https://w3id.org/citydata/21972/v1/"
     xmlns:cdm1="https://w3id.org/citydata/part1/v1/">
    <owl:Ontology rdf:about="https://w3id.org/citydata/part2/v1/InfrastructurePattern/">
        <!-- Identity -->
        <dcterms:title>Information technology - City data model - Part 2: City level concepts - Infrastructure pattern</dcterms:title>
        <rdfs:seeAlso rdf:resource="https://www.iso.org/standard/80742.html"/>
        <dcterms:bibliographicCitation>ISO/IEC 5087-2:2024</dcterms:bibliographicCitation>
    	<skos:definition>This ontology specifies the city-level concepts for the infrastructure pattern of the city data model. The Infrastructure pattern defines the concepts needed to capture various types of city infrastructure, such as buildings and roads. The Infrastructure pattern reuses the Spatial Location pattern (from ISO 5087-1) in order to capture the location of these infrastructure elements.</skos:definition>
    	<vann:preferredNamespaceUri>https://w3id.org/citydata/part2/v1/</vann:preferredNamespaceUri>
    	<vann:preferredNamespacePrefix>cdm2</vann:preferredNamespacePrefix>

    	<!-- Provenance -->
        <dcterms:creator>Megan Katsumi</dcterms:creator>
        <dcterms:creator>Mark Fox</dcterms:creator>
    	<dcterms:creator>Kenneth Vaughn</dcterms:creator>
        <!-- Prior release -->
        <rdfs:comment>The prior version of this ontology used a different ontology IRI. This update remains semantically consistent with the version adopted as ISO 5087-2:2024.</rdfs:comment>
        <owl:priorVersion rdf:resource="https://standards.iso.org/iso-iec/5087/-2/ed-1/en/ontology/Infrastructure/"/>
        <!-- This release -->
		<dcterms:modified rdf:datatype="http://www.w3.org/2001/XMLSchema#date">2026-02-12</dcterms:modified> 
        <owl:versionInfo>1.3.0</owl:versionInfo>
        <owl:versionIRI rdf:resource="https://w3id.org/citydata/part2/v1/InfrastructurePattern/r3.0/"/>
        
        <!-- License -->
        <cc:license>http://creativecommons.org/licenses/by/4.0/</cc:license>
        
        <!-- Imports -->
        <owl:imports rdf:resource="https://w3id.org/citydata/part2/v1/ContactPattern/"/>
    </owl:Ontology>

    
    <!-- 
    ///////////////////////////////////////////////////////////////////////////////////////
    //
    // Classes
    //
    ///////////////////////////////////////////////////////////////////////////////////////
     -->

    
    <!-- https://w3id.org/citydata/part2/v1/InfrastructureThing -->

    <owl:Class rdf:about="https://w3id.org/citydata/part2/v1/InfrastructureThing">
        <rdfs:subClassOf rdf:resource="https://w3id.org/citydata/part2/v1/CityThing"/>
        <skos:definition>Added for organizational purposes, to identify classes defined in the Infrastructure pattern.</skos:definition>
    </owl:Class>
    

    <!-- https://w3id.org/citydata/part2/v1/InfrastructureElement -->

    <owl:Class rdf:about="https://w3id.org/citydata/part2/v1/InfrastructureElement">
        <skos:definition>An Infrastructure Element is a generic representation of a city structure of interest.</skos:definition>
        <rdfs:subClassOf rdf:resource="https://w3id.org/citydata/part2/v1/InfrastructureThing"/>
        <rdfs:subClassOf>
            <owl:Restriction>
                <owl:onProperty rdf:resource="https://w3id.org/citydata/21972/v1/hasValue"/>
                <owl:allValuesFrom rdf:resource="https://w3id.org/citydata/part1/v1/MonetaryValue"/>
            </owl:Restriction>
        </rdfs:subClassOf>
        <rdfs:subClassOf>
            <owl:Restriction>
                <owl:onProperty rdf:resource="https://w3id.org/citydata/part1/v1/hasProperPart"/>
                <owl:allValuesFrom rdf:resource="https://w3id.org/citydata/part2/v1/InfrastructureElement"/>
            </owl:Restriction>
        </rdfs:subClassOf>
        <rdfs:subClassOf>
            <owl:Restriction>
                <owl:onProperty rdf:resource="https://w3id.org/citydata/part1/v1/hasLocation"/>
                <owl:allValuesFrom rdf:resource="https://w3id.org/citydata/part1/v1/Location"/>
            </owl:Restriction>
        </rdfs:subClassOf>
        <rdfs:subClassOf>
            <owl:Restriction>
                <owl:onProperty rdf:resource="https://w3id.org/citydata/part2/v1/hasAddress"/>
                <owl:allValuesFrom rdf:resource="https://w3id.org/citydata/part2/v1/Address"/>
            </owl:Restriction>
        </rdfs:subClassOf>
        <rdfs:subClassOf>
            <owl:Restriction>
                <owl:onProperty rdf:resource="https://w3id.org/citydata/part1/v1/hasDescription"/>
                <owl:allValuesFrom rdf:resource="http://www.w3.org/2001/XMLSchema#string"/>
            </owl:Restriction>
        </rdfs:subClassOf>
        <rdfs:subClassOf>
            <owl:Restriction>
                <owl:onProperty rdf:resource="https://w3id.org/citydata/part1/v1/hasIdentifier"/>
                <owl:allValuesFrom rdf:resource="http://www.w3.org/2001/XMLSchema#string"/>
            </owl:Restriction>
        </rdfs:subClassOf>
        <rdfs:subClassOf>
            <owl:Restriction>
                <owl:onProperty rdf:resource="https://w3id.org/citydata/part1/v1/hasName"/>
                <owl:allValuesFrom rdf:resource="http://www.w3.org/2001/XMLSchema#string"/>
            </owl:Restriction>
        </rdfs:subClassOf>
    </owl:Class>
    

</rdf:RDF>
