<?xml version="1.0"?>
<rdf:RDF xmlns="https://w3id.org/isoiec5087-2/v1/"
     xml:base="https://w3id.org/isoiec5087-2/v1/"
     xmlns:cc="http://creativecommons.org/ns#"
     xmlns:dcterms="http://purl.org/dc/terms/"
     xmlns:owl="http://www.w3.org/2002/07/owl#"
     xmlns:rdf="http://www.w3.org/1999/02/22-rdf-syntax-ns#"
     xmlns:rdfs="http://www.w3.org/2000/01/rdf-schema#"
     xmlns:skos="http://www.w3.org/2004/02/skos/core#"
     xmlns:vann="http://purl.org/vocab/vann/"
     xmlns:xml="http://www.w3.org/XML/1998/namespace"
     xmlns:xsd="http://www.w3.org/2001/XMLSchema#"
     xmlns:i72="https://w3id.org/isoiec21972/v1/"
     xmlns:cdm1="https://w3id.org/isoiec5087-1/v1/">
    <owl:Ontology rdf:about="https://w3id.org/isoiec5087-2/v1/LandUsePattern">
        <!-- Identity -->
        <dcterms:title>Information technology - City data model - Part 2: City level concepts - Land Use pattern</dcterms:title>
        <rdfs:seeAlso rdf:resource="https://www.iso.org/standard/80742.html"/>
        <dcterms:bibliographicCitation>ISO/IEC 5087-2:2024</dcterms:bibliographicCitation>
    	<skos:definition>This ontology specifies the city-level concepts for the land use pattern of the city data model. The Land Use Pattern captures concepts related to land use and cover over time. Land Use Classifications provide a means of describing the land cover/use in a standard way. Various classification systems are used to identify types of land use. Currently, we include LBCS, CLUMP, and AAFC. The ontology reuses and extends the Land Based Classification Standards (LBCS) Ontology  presented by (Montenegro, Gomes, Urbano, and Duarte, 2011) for this purpose.</skos:definition>
    	<vann:preferredNamespaceUri>https://w3id.org/isoiec5087-2/v1/</vann:preferredNamespaceUri>
    	<vann:preferredNamespacePrefix>cdm2</vann:preferredNamespacePrefix>

    	<!-- Provenance -->
        <dcterms:creator>Megan Katsumi</dcterms:creator>
        <dcterms:creator>Mark Fox</dcterms:creator>
    	<dcterms:creator>Kenneth Vaughn</dcterms:creator>
        <dcterms:issued rdf:datatype="http://www.w3.org/2001/XMLSchema#date">2024</dcterms:issued> <!-- Date of the source document, comment out if draft -->
        <owl:priorVersion rdf:resource="https://standards.iso.org/iso-iec/5087/-2/ed-1/en/ontology/LandUse/"/>
        <owl:priorVersion rdf:datatype="http://www.w3.org/2001/XMLSchema#date">2021-01-11</owl:priorVersion> <!-- Date of prior ontology file, if any -->
		<dcterms:modified rdf:datatype="http://www.w3.org/2001/XMLSchema#date">2026-02-08</dcterms:modified> <!-- Date of this ontology file -->
        <owl:versionInfo>1.3.0</owl:versionInfo>
        <owl:versionIRI rdf:resource="https://w3id.org/isoiec5087-2/v1/r3.0"/>
        <rdfs:comment>The prior version of this ontology used a different ontology IRI. This update remains semantically consistent with the version adopted as ISO 5087-2:2024.</rdfs:comment>
        
        <!-- License -->
        <cc:license>http://creativecommons.org/licenses/by/4.0/</cc:license>
        
        <!-- Imports -->
        <owl:imports rdf:resource="https://w3id.org/isoiec5087-2/v1/CodePattern"/>
    </owl:Ontology>
    

    <!-- 
    ///////////////////////////////////////////////////////////////////////////////////////
    //
    // Object Properties
    //
    ///////////////////////////////////////////////////////////////////////////////////////
     -->
    

    <!-- https://w3id.org/isoiec5087-2/v1/LandUseObjectProperty -->
    <owl:ObjectProperty rdf:about="https://w3id.org/isoiec5087-2/v1/LandUseObjectProperty">
        <skos:definition>Added for organizational purposes, to identify object properties defined in the Land Use ontology.</skos:definition>
        <rdfs:subPropertyOf rdf:resource="https://w3id.org/isoiec5087-2/v1/CityObjectProperty"/>
    </owl:ObjectProperty>
   

    <!-- https://w3id.org/isoiec5087-2/v1/hasArea -->

    <owl:ObjectProperty rdf:about="https://w3id.org/isoiec5087-2/v1/hasArea">
        <skos:definition>identifies the size of a Land Area</skos:definition>
        <rdfs:subPropertyOf rdf:resource="https://w3id.org/isoiec5087-2/v1/LandUseObjectProperty"/>
        <rdfs:domain rdf:resource="https://w3id.org/isoiec5087-2/v1/LandArea"/>
        <rdfs:range rdf:resource="https://w3id.org/isoiec5087-1/v1/Area"/>
    </owl:ObjectProperty>
    

    <!-- https://w3id.org/isoiec5087-2/v1/hasLandArea -->

    <owl:ObjectProperty rdf:about="https://w3id.org/isoiec5087-2/v1/hasLandArea">
        <skos:definition>Identifies the spatial area occupied by the object.</skos:definition>
        <rdfs:subPropertyOf rdf:resource="https://w3id.org/isoiec5087-2/v1/LandUseObjectProperty"/>
        <rdfs:range rdf:resource="https://w3id.org/isoiec5087-2/v1/LandArea"/>
    </owl:ObjectProperty>


    <!-- Issue: v1.2.0 called "hasPopulation" hasPopulationSize. Reverted to "hasPopulation" for consistency with ISO/IEC 5087-2. -->
    <!-- https://w3id.org/isoiec5087-2/v1/hasPopulation -->

    <owl:ObjectProperty rdf:about="https://w3id.org/isoiec5087-2/v1/hasPopulation">
        <skos:definition>Specifies the number of people living in the LandArea.</skos:definition>
        <rdfs:subPropertyOf rdf:resource="https://w3id.org/isoiec5087-2/v1/LandUseObjectProperty"/>
        <rdfs:domain rdf:resource="https://w3id.org/isoiec5087-2/v1/LandArea"/>
        <rdfs:range rdf:resource="https://w3id.org/isoiec21972/v1/Population"/>
    </owl:ObjectProperty>
    

    <!-- https://w3id.org/isoiec5087-2/v1/landUse -->

    <owl:ObjectProperty rdf:about="https://w3id.org/isoiec5087-2/v1/landUse">
        <skos:definition>Identifies a Land Use Classification that is identified for the Land Area.</skos:definition>
        <rdfs:subPropertyOf rdf:resource="https://w3id.org/isoiec5087-2/v1/LandUseObjectProperty"/>
        <rdfs:domain rdf:resource="https://w3id.org/isoiec5087-2/v1/LandArea"/>
        <rdfs:range rdf:resource="https://w3id.org/isoiec5087-2/v1/LandUseClassification"/>
    </owl:ObjectProperty>
    

    <!-- 
    ///////////////////////////////////////////////////////////////////////////////////////
    //
    // Classes
    //
    ///////////////////////////////////////////////////////////////////////////////////////
     -->

    
    <!-- https://w3id.org/isoiec5087-2/v1/LandUseThing -->

    <owl:Class rdf:about="https://w3id.org/isoiec5087-2/v1/LandUseThing">
        <rdfs:subClassOf rdf:resource="https://w3id.org/isoiec5087-2/v1/CityThing"/>
        <skos:definition>Added for organizational purposes, to identify classes defined in the Land Use ontology.</skos:definition>
    </owl:Class>
    

    <!-- https://w3id.org/isoiec5087-2/v1/LandArea -->

    <owl:Class rdf:about="https://w3id.org/isoiec5087-2/v1/LandArea">
        <skos:definition>A Land Area is a defined geographic area of land.</skos:definition>
        <!-- Issue: ISO/IEC 5087-2 defines LandArea to have a location (hasLocation) rather than being a type of location. Recommend keeping as type of location. -->
        <rdfs:subClassOf rdf:resource="https://w3id.org/isoiec5087-1/v1/Location"/>
        <rdfs:subClassOf rdf:resource="https://w3id.org/isoiec5087-2/v1/LandUseThing"/>
        <rdfs:subClassOf>
            <owl:Restriction>
                <owl:onProperty rdf:resource="https://w3id.org/isoiec5087-2/v1/hasArea"/>
                <owl:allValuesFrom rdf:resource="https://w3id.org/isoiec5087-1/v1/Area"/>
            </owl:Restriction>
        </rdfs:subClassOf>
        <!-- Issue: ISO/IEC 5087-2 defines LandArea.landUse as min 1 rather than only. Recommend keeping only for unrestricted areas. -->
        <rdfs:subClassOf>
            <owl:Restriction>
                <owl:onProperty rdf:resource="https://w3id.org/isoiec5087-2/v1/landUse"/>
                <owl:allValuesFrom rdf:resource="https://w3id.org/isoiec5087-2/v1/LandUseClassification"/>
            </owl:Restriction>
        </rdfs:subClassOf>
        <rdfs:subClassOf>
            <owl:Restriction>
                <owl:onProperty rdf:resource="https://w3id.org/isoiec5087-2/v1/hasPopulation"/>
                <owl:allValuesFrom rdf:resource="https://w3id.org/isoiec21972/v1/Population"/>
            </owl:Restriction>
        </rdfs:subClassOf>
        <!-- Issue: ISO/IEC 5087-2 does not define LandArea.hasDescription. Recommend keeping. -->
        <rdfs:subClassOf>
            <owl:Restriction>
                <owl:onProperty rdf:resource="https://w3id.org/isoiec5087-1/v1/hasDescription"/>
                <owl:allValuesFrom rdf:resource="http://www.w3.org/2001/XMLSchema#string"/>
            </owl:Restriction>
        </rdfs:subClassOf>
    </owl:Class>
    

    <!-- https://w3id.org/isoiec5087-2/v1/LandUseClassification -->

    <owl:Class rdf:about="https://w3id.org/isoiec5087-2/v1/LandUseClassification">
        <skos:definition>Land Use Classification is a type of Code that describes the use of a Land Area.</skos:definition>
        <skos:note>Land Use Classifications provide a means of describing the use in a standard way. Various classification systems are used to identify types of land use, such as LBCS, CLUMP, and AAFC.</skos:note>
        <rdfs:subClassOf rdf:resource="https://w3id.org/isoiec5087-2/v1/LandUseThing"/>
        <rdfs:subClassOf>
            <owl:Restriction>
                <owl:onProperty rdf:resource="https://w3id.org/isoiec5087-2/v1/hasCode"/>
                <owl:allValuesFrom rdf:resource="https://w3id.org/isoiec5087-2/v1/Code"/>
            </owl:Restriction>
        </rdfs:subClassOf>
    </owl:Class>
    

</rdf:RDF>
