<?xml version="1.0"?>
<rdf:RDF xmlns="https://w3id.org/citydata/part2/v1/"
     xml:base="https://w3id.org/citydata/part2/v1/"
     xmlns:cc="http://creativecommons.org/ns#"
     xmlns:dcterms="http://purl.org/dc/terms/"
     xmlns:owl="http://www.w3.org/2002/07/owl#"
     xmlns:rdf="http://www.w3.org/1999/02/22-rdf-syntax-ns#"
     xmlns:rdfs="http://www.w3.org/2000/01/rdf-schema#"
     xmlns:skos="http://www.w3.org/2004/02/skos/core#"
     xmlns:vann="http://purl.org/vocab/vann/"
     xmlns:xml="http://www.w3.org/XML/1998/namespace"
     xmlns:xsd="http://www.w3.org/2001/XMLSchema#"
     xmlns:cdm1="https://w3id.org/citydata/part1/v1/">
    <owl:Ontology rdf:about="https://w3id.org/citydata/part2/v1/TransportInfrastructurePattern/">
        <!-- Identity -->
        <dcterms:title>Information technology - City data model - Part 2: City level concepts - Transport Infrastructure pattern</dcterms:title>
        <rdfs:seeAlso rdf:resource="https://www.iso.org/standard/80742.html"/>
        <dcterms:bibliographicCitation>ISO/IEC 5087-2:2024</dcterms:bibliographicCitation>
    	<skos:definition>This ontology specifies the city-level concepts for the transport infrastructure pattern of the city data model. The Transportation Infrastructure pattern defines the concepts that are relevant in describing the physical transportation infrastructure and their characteristics. This includes the concepts of a Road, Bridge, and Tunnel. The Infrastructure Pattern is reused here, as these transportation structures are all defined as types of (subclasses) Infrastructure Elements.</skos:definition>
    	<vann:preferredNamespaceUri>https://w3id.org/citydata/part2/v1/</vann:preferredNamespaceUri>
    	<vann:preferredNamespacePrefix>cdm2</vann:preferredNamespacePrefix>

    	<!-- Provenance -->
        <dcterms:creator>Megan Katsumi</dcterms:creator>
        <dcterms:creator>Mark Fox</dcterms:creator>
    	<dcterms:creator>Kenneth Vaughn</dcterms:creator>
        <!-- Prior release -->
        <rdfs:comment>The prior version of this ontology used a different ontology IRI. This update remains semantically consistent with the version adopted as ISO 5087-2:2024.</rdfs:comment>
        <owl:priorVersion rdf:resource="https://standards.iso.org/iso-iec/5087/-2/ed-1/en/ontology/TransportInfrastructure/"/>
        <!-- This release -->
		<dcterms:modified rdf:datatype="http://www.w3.org/2001/XMLSchema#date">2026-02-12</dcterms:modified> 
        <owl:versionInfo>1.3.0</owl:versionInfo>
        <owl:versionIRI rdf:resource="https://w3id.org/citydata/part2/v1/TransportInfrastructurePattern/r3.0/"/>
        
        <!-- License -->
        <cc:license>http://creativecommons.org/licenses/by/4.0/</cc:license>
        
        <!-- Imports -->
        <owl:imports rdf:resource="https://w3id.org/citydata/part2/v1/InfrastructurePattern/"/>
    </owl:Ontology>
    

    <!-- 
    ///////////////////////////////////////////////////////////////////////////////////////
    //
    // Object Properties
    //
    ///////////////////////////////////////////////////////////////////////////////////////
     -->

    
    <!-- https://w3id.org/citydata/part2/v1/TransportInfrastructureObjectProperty -->

    <owl:ObjectProperty rdf:about="https://w3id.org/citydata/part2/v1/TransportInfrastructureObjectProperty">
        <skos:definition>Added for organizational purposes, to identify object properties defined for the Transport Infrastructure Pattern in the City-level CDM ontology.</skos:definition>
        <rdfs:subPropertyOf rdf:resource="https://w3id.org/citydata/part2/v1/CityObjectProperty"/>
    </owl:ObjectProperty>


    <!-- https://w3id.org/citydata/part2/v1/networkType -->

    <owl:ObjectProperty rdf:about="https://w3id.org/citydata/part2/v1/networkType">
        <skos:definition>Identifies the type of network.</skos:definition>
        <rdfs:comment xml:lang="en">This was originally defined for types of transport infrastructure but can be applied to other network types as well.</rdfs:comment>
        <rdfs:subPropertyOf rdf:resource="https://w3id.org/citydata/part2/v1/TransportInfrastructureObjectProperty"/>
        <rdfs:range rdf:resource="https://w3id.org/citydata/part2/v1/Code"/>
    </owl:ObjectProperty>
    

    <!-- https://w3id.org/citydata/part2/v1/supports -->

    <owl:ObjectProperty rdf:about="https://w3id.org/citydata/part2/v1/supports">
        <skos:definition>Identifies the infrastructure element that is supported (carried in or carried through) the current (domain) object.</skos:definition>
        <skos:example>A road segment can be supported by a tunnel or bridge.</skos:example>
        <rdfs:subPropertyOf rdf:resource="https://w3id.org/citydata/part2/v1/TransportInfrastructureObjectProperty"/>
        <rdfs:range rdf:resource="https://w3id.org/citydata/part2/v1/InfrastructureElement"/>
    </owl:ObjectProperty>
    

    <!-- 
    ///////////////////////////////////////////////////////////////////////////////////////
    //
    // Classes
    //
    ///////////////////////////////////////////////////////////////////////////////////////
     -->

    
    <!-- https://w3id.org/citydata/part2/v1/TransportInfrastructureThing -->
     <owl:Class rdf:about="https://w3id.org/citydata/part2/v1/TransportInfrastructureThing">
        <rdfs:subClassOf rdf:resource="https://w3id.org/citydata/part2/v1/CityPatternThing"/>
        <skos:definition>Added for organizational purposes, to identify classes defined in the Transport Infrastructure Pattern ontology.</skos:definition>
    </owl:Class>
    

    <!-- https://w3id.org/citydata/part2/v1/Bridge -->

    <owl:Class rdf:about="https://w3id.org/citydata/part2/v1/Bridge">
        <skos:definition>A Bridge is a Infrastructure Element that enables travel over some obstacle or area. It may contain some Road Segments or Rail Line Segments.</skos:definition>
        <skos:note>A Bridge is identified as such by a governing body.</skos:note>
        <rdfs:subClassOf rdf:resource="https://w3id.org/citydata/part2/v1/InfrastructureElement"/>
        <rdfs:subClassOf>
            <owl:Restriction>
                <owl:onProperty rdf:resource="https://w3id.org/citydata/part1/v1/hasProperPart"/>
                <owl:allValuesFrom rdf:resource="https://w3id.org/citydata/part2/v1/BridgeSegment"/>
            </owl:Restriction>
        </rdfs:subClassOf>
        <rdfs:subClassOf>
            <owl:Restriction>
                <owl:onProperty rdf:resource="https://w3id.org/citydata/part2/v1/supports"/>
                <owl:allValuesFrom rdf:resource="https://w3id.org/citydata/part2/v1/TravelledWaySegment"/>
            </owl:Restriction>
        </rdfs:subClassOf>
    </owl:Class>
    

    <!-- https://w3id.org/citydata/part2/v1/BridgeSegment -->

    <owl:Class rdf:about="https://w3id.org/citydata/part2/v1/BridgeSegment">
        <rdfs:subClassOf rdf:resource="https://w3id.org/citydata/part2/v1/InfrastructureElement"/>
        <rdfs:subClassOf>
            <owl:Restriction>
                <owl:onProperty rdf:resource="https://w3id.org/citydata/part2/v1/supports"/>
                <owl:allValuesFrom rdf:resource="https://w3id.org/citydata/part2/v1/TravelledWaySegment"/>
            </owl:Restriction>
        </rdfs:subClassOf>
    </owl:Class>
    

    <!-- https://w3id.org/citydata/part2/v1/RailLine -->

    <owl:Class rdf:about="https://w3id.org/citydata/part2/v1/RailLine">
        <skos:definition>A Rail Line is a type of Travelled Way that describes a part of the physical transportation infrastructure that has been fitted with tracks to allow travel by trains and other sorts of rail vehicles. No distinction is made between Rail Line types at this level.</skos:definition>
        <rdfs:subClassOf rdf:resource="https://w3id.org/citydata/part2/v1/TravelledWay"/>
        <rdfs:subClassOf>
            <owl:Restriction>
                <owl:onProperty rdf:resource="https://w3id.org/citydata/part1/v1/aggregationOf"/>
                <owl:allValuesFrom rdf:resource="https://w3id.org/citydata/part2/v1/RailLink"/>
            </owl:Restriction>
        </rdfs:subClassOf>
    </owl:Class>
    

    <!-- https://w3id.org/citydata/part2/v1/RailSegment -->

    <owl:Class rdf:about="https://w3id.org/citydata/part2/v1/RailSegment">
        <skos:definition>A Rail Segment is a type of Travelled Way Segment that represents part of a Rail Link.</skos:definition>
        <rdfs:subClassOf rdf:resource="https://w3id.org/citydata/part2/v1/TravelledWaySegment"/>
        <rdfs:subClassOf>
            <owl:Restriction>
                <owl:onProperty rdf:resource="https://w3id.org/citydata/part1/v1/properPartOf"/>
                <owl:someValuesFrom rdf:resource="https://w3id.org/citydata/part2/v1/RailLink"/>
            </owl:Restriction>
        </rdfs:subClassOf>
    </owl:Class>
    

    <!-- https://w3id.org/citydata/part2/v1/Road -->

    <owl:Class rdf:about="https://w3id.org/citydata/part2/v1/Road">
        <skos:definition>A Road is a type of Travelled Way that describes a part of the physical transport infrastructure that has been improved to allow travel by motor vehicles, persons, bicycles, or similar methods of conveyance. road vehicles. No distinction is made between Road types at this level.</skos:definition>
        <rdfs:subClassOf rdf:resource="https://w3id.org/citydata/part2/v1/TravelledWay"/>
        <rdfs:subClassOf>
            <owl:Restriction>
                <owl:onProperty rdf:resource="https://w3id.org/citydata/part1/v1/aggregationOf"/>
                <owl:allValuesFrom rdf:resource="https://w3id.org/citydata/part2/v1/RoadLink"/>
            </owl:Restriction>
        </rdfs:subClassOf>
    </owl:Class>
    

    <!-- https://w3id.org/citydata/part2/v1/RoadSegment -->

    <owl:Class rdf:about="https://w3id.org/citydata/part2/v1/RoadSegment">
        <skos:definition>A Road Segment is a type of Travelled Way Segment that represents part of a Road Link.</skos:definition>
        <rdfs:subClassOf rdf:resource="https://w3id.org/citydata/part2/v1/TravelledWaySegment"/>
        <rdfs:subClassOf>
            <owl:Restriction>
                <owl:onProperty rdf:resource="https://w3id.org/citydata/part1/v1/properPartOf"/>
                <owl:someValuesFrom rdf:resource="https://w3id.org/citydata/part2/v1/RoadLink"/>
            </owl:Restriction>
        </rdfs:subClassOf>
        <rdfs:subClassOf>
            <owl:Restriction>
                <owl:onProperty rdf:resource="https://w3id.org/citydata/part2/v1/networkType"/>
                <owl:allValuesFrom rdf:resource="https://w3id.org/citydata/part2/v1/RoadNetworkType"/>
            </owl:Restriction>
        </rdfs:subClassOf>
    </owl:Class>
    

    <!-- https://w3id.org/citydata/part2/v1/Tunnel -->

    <owl:Class rdf:about="https://w3id.org/citydata/part2/v1/Tunnel">
        <skos:definition>A Tunnel is a Infrastructure Element that enables travel through or underneath some obstacle or area. It may contain some Road or RailLine Segments.</skos:definition>
        <rdfs:subClassOf rdf:resource="https://w3id.org/citydata/part2/v1/InfrastructureElement"/>
        <rdfs:subClassOf>
            <owl:Restriction>
                <owl:onProperty rdf:resource="https://w3id.org/citydata/part1/v1/hasProperPart"/>
                <owl:allValuesFrom rdf:resource="https://w3id.org/citydata/part2/v1/TunnelSegment"/>
            </owl:Restriction>
        </rdfs:subClassOf>
        <rdfs:subClassOf>
            <owl:Restriction>
                <owl:onProperty rdf:resource="https://w3id.org/citydata/part2/v1/supports"/>
                <owl:allValuesFrom rdf:resource="https://w3id.org/citydata/part2/v1/TravelledWaySegment"/>
            </owl:Restriction>
        </rdfs:subClassOf>
    </owl:Class>
    

    <!-- https://w3id.org/citydata/part2/v1/TunnelSegment -->

    <owl:Class rdf:about="https://w3id.org/citydata/part2/v1/TunnelSegment">
        <skos:definition>A Tunnel Segment is a type of Infrastructure Element that represents part of a Tunnel.</skos:definition>
        <rdfs:subClassOf rdf:resource="https://w3id.org/citydata/part2/v1/InfrastructureElement"/>
        <rdfs:subClassOf>
            <owl:Restriction>
                <owl:onProperty rdf:resource="https://w3id.org/citydata/part2/v1/supports"/>
                <owl:allValuesFrom rdf:resource="https://w3id.org/citydata/part2/v1/TravelledWaySegment"/>
            </owl:Restriction>
        </rdfs:subClassOf>
    </owl:Class>
    

    <!-- https://w3id.org/citydata/part2/v1/RailLink -->

    <owl:Class rdf:about="https://w3id.org/citydata/part2/v1/RailLink">
        <skos:definition>A Rail Link is a type of Travelled Way Link that represents a length of RailLine.</skos:definition>
        <rdfs:subClassOf rdf:resource="https://w3id.org/citydata/part2/v1/TravelledWayLink"/>
        <rdfs:subClassOf>
            <owl:Restriction>
                <owl:onProperty rdf:resource="https://w3id.org/citydata/part1/v1/aggregateOf"/>
                <owl:allValuesFrom rdf:resource="https://w3id.org/citydata/part2/v1/RailLine"/>
            </owl:Restriction>
        </rdfs:subClassOf>
    </owl:Class>
    

    <!-- https://w3id.org/citydata/part2/v1/RoadLink -->

    <owl:Class rdf:about="https://w3id.org/citydata/part2/v1/RoadLink">
        <skos:definition>A Road Link is a type of Travelled Way Link that represents a length of Road.</skos:definition>
        <rdfs:subClassOf rdf:resource="https://w3id.org/citydata/part2/v1/TravelledWayLink"/>
        <rdfs:subClassOf>
            <owl:Restriction>
                <owl:onProperty rdf:resource="https://w3id.org/citydata/part1/v1/aggregateOf"/>
                <owl:allValuesFrom rdf:resource="https://w3id.org/citydata/part2/v1/Road"/>
            </owl:Restriction>
        </rdfs:subClassOf>
    </owl:Class>
    

    <!-- https://w3id.org/citydata/part2/v1/RoadNetworkType -->

    <owl:Class rdf:about="https://w3id.org/citydata/part2/v1/RoadNetworkType">
        <rdfs:subClassOf rdf:resource="https://w3id.org/citydata/part2/v1/InfrastructureThing"/>
        <rdfs:subClassOf>
            <owl:Restriction>
                <owl:onProperty rdf:resource="https://w3id.org/citydata/part2/v1/hasCode"/>
                <owl:allValuesFrom rdf:resource="https://w3id.org/citydata/part2/v1/Code"/>
            </owl:Restriction>
        </rdfs:subClassOf>
    </owl:Class>
    

    <!-- https://w3id.org/citydata/part2/v1/TravelledWay -->

    <owl:Class rdf:about="https://w3id.org/citydata/part2/v1/TravelledWay">
        <skos:definition>A Travelled Way is a type of Infrastructure Element that enables travel.</skos:definition>
        <rdfs:subClassOf rdf:resource="https://w3id.org/citydata/part2/v1/InfrastructureElement"/>
        <rdfs:subClassOf>
            <owl:Restriction>
                <owl:onProperty rdf:resource="https://w3id.org/citydata/part1/v1/aggregationOf"/>
                <owl:allValuesFrom rdf:resource="https://w3id.org/citydata/part2/v1/TravelledWayLink"/>
            </owl:Restriction>
        </rdfs:subClassOf>
    </owl:Class>
    

    <!-- https://w3id.org/citydata/part2/v1/TravelledWayLink -->

    <owl:Class rdf:about="https://w3id.org/citydata/part2/v1/TravelledWayLink">
        <skos:definition>A Travelled Way Link represents a continuous length of a Travelled Way and is a type of Infrastructure Element that connects two or more Travelled Way Segments.</skos:definition>
        <rdfs:subClassOf rdf:resource="https://w3id.org/citydata/part2/v1/InfrastructureElement"/>
        <rdfs:subClassOf>
            <owl:Restriction>
                <owl:onProperty rdf:resource="https://w3id.org/citydata/part1/v1/aggregateOf"/>
                <owl:allValuesFrom rdf:resource="https://w3id.org/citydata/part2/v1/TravelledWay"/>
            </owl:Restriction>
        </rdfs:subClassOf>
    </owl:Class>
    

    <!-- https://w3id.org/citydata/part2/v1/TravelledWaySegment -->

    <owl:Class rdf:about="https://w3id.org/citydata/part2/v1/TravelledWaySegment">
        <skos:definition>A Travelled Way Segment is a type of Infrastructure Element that represents part of a Travelled Way Link.</skos:definition>
        <rdfs:subClassOf rdf:resource="https://w3id.org/citydata/part2/v1/InfrastructureElement"/>
        <rdfs:subClassOf>
            <owl:Restriction>
                <owl:onProperty rdf:resource="https://w3id.org/citydata/part1/v1/aggregateOf"/>
                <owl:someValuesFrom rdf:resource="https://w3id.org/citydata/part2/v1/TravelledWayLink"/>
            </owl:Restriction>
        </rdfs:subClassOf>
    </owl:Class>


</rdf:RDF>
